

1. Find the **first five nonzero terms** of the power series solution about $x_0 = 2$ of the initial value problem:

$$\begin{cases} y'' + 2xy' - y = 0, \\ y(2) = 1, \quad y'(2) = -1. \end{cases}$$

[15]

2. Consider the following equation:

$$(x+3)^2 y'' - 5(x+3)y' + 9y = 0.$$

- (a) Identify all the ordinary and singular points; and for singular point(s), identify the type of regular singular or irregular singular point(s). Explain your reasons.
(b) Find the general solution of the equation.

[5]

[10]

3. Use Laplace transform to solve the initial value problem:

$$y''(t) + 4y(t) = f(t) + \delta(t - 1.5); \quad y(0) = 0, \quad y'(0) = 0;$$

where

$$f(t) = \begin{cases} 0 & 0 \leq t < 4 \\ (t-4)/6, & 4 \leq t < 10, \\ 1, & t \geq 10. \end{cases}$$

[20]

4. Apply the **Laplace transform** to solve the initial value problem:

$$2y'' + y' + 2y = e^{2t}, \quad y(0) = 0, \quad y'(0) = 1.$$

[15]

5. Solve the initial value problem:

$$x' = \begin{pmatrix} -1/2 & 1 \\ -1 & -1/2 \end{pmatrix} x; \quad x(0) = \begin{pmatrix} 1 \\ -1 \end{pmatrix}.$$

[15]

6. Consider the initial value problem:

$$y'' + y' - 6y = 0; \quad y(0) = 3, \quad y'(0) = 0.$$

- (a) Transform the problem into an initial value problem of first-order system of equations.
(b) Solve the initial value problem obtained in (a) using the method for systems of first-order equations.
(c) Find the solution y of the original initial value problem through the results obtained in (a) and (b).

[20]

— End —

1. Find the first five nonzero terms of the power series solution about $x_0 = 2$ of the initial value problem:

$$\begin{cases} y'' + 2xy' - y = 0, \\ y(2) = 1, \quad y'(2) = -1. \end{cases}$$

[15]

Since $P(x) = 1$, $x = 2$ is a regular point

Assume $y = \sum_{n=0}^{\infty} a_n (x-2)^n$

Then $y' = \sum_{n=1}^{\infty} n a_n (x-2)^{n-1} = \sum_{n=0}^{\infty} (n+1) a_{n+1} (x-2)^n$ 2'

$$y'' = \sum_{n=1}^{\infty} n(n+1) a_{n+1} (x-2)^{n-1} = \sum_{n=0}^{\infty} (n+1)(n+2) a_{n+2} (x-2)^n$$

$$2xy' = 2(x-2)y' + 4y' = 2 \sum_{n=0}^{\infty} n a_n (x-2)^n + 4 \sum_{n=0}^{\infty} (n+1) a_{n+1} (x-2)^n$$
 5'

$$\Rightarrow y'' + 2xy' - y = \sum_{n=0}^{\infty} [(n+2)(n+1) a_{n+2} + 4(n+1) a_{n+1} + 2n a_n - a_n] (x-2)^n = 0$$

$$\Rightarrow (n+2)(n+1) a_{n+2} + 4(n+1) a_{n+1} + (2n-1) a_n = 0$$

$$n=0: 2a_2 + 4a_1 - a_0 = 0 \Rightarrow a_2 = \frac{1}{2}a_0 - a_1$$
 3'

$$n=1: 6a_3 + 8a_2 + a_1 = 0 \Rightarrow a_3 = -\frac{2}{3}a_0 + \frac{5}{2}a_1$$

$$n=2: 12a_4 + 12a_3 + 3a_2 = 0 \Rightarrow a_4 = \frac{13}{24}a_0 - 2a_1$$

Since $a_0 = y(2) = 1$, $a_1 = y'(2) = -1$

then $a_2 = \frac{3}{2}$, $a_3 = -\frac{19}{6}$, $a_4 = \frac{61}{24}$ 3'

Therefore,

$$y = 1 - (x-2) + \frac{3}{2}(x-2)^2 - \frac{19}{6}(x-2)^3 + \frac{61}{24}(x-2)^4 + \dots$$
 2' □

2. Consider the following equation:

$$(x+3)^2 y'' - 5(x+3)y' + 9y = 0.$$

- (a) Identify all the ordinary and singular points; and for singular point(s), identify the type of regular singular or irregular singular point(s). Explain your reasons.

[5]

- (b) Find the general solution of the equation.

[10]

Solution. (a) $P(x) = (x+3)^2$, $Q(x) = -5(x+3)$, $R(x) = 9$.

P, Q, R are polynomials with no common factors.

Let $P(x) = 0$, we have $x_0 = -3$, which is a singular point

Let $P(x) \neq 0$, we have $x_0 \neq -3$, so ordinary points are $\{x | x \neq -3\}$.

$$\text{For } x_0 = -3, \lim_{x \rightarrow x_0} (x - x_0) \frac{Q(x)}{P(x)} = -5$$

$$\lim_{x \rightarrow x_0} (x - x_0)^2 \frac{R(x)}{P(x)} = 9. \quad \text{are finite}$$

so $x_0 = -3$ is a regular singular point.

(b). This is an Euler equation.

The corresponding characteristic equation is

$$r^2 + (-5-1)r + 9 = 0$$

$$r_1 = r_2 = 3$$

So the general solution is

$$y = c_1 |x+3|^3 + c_2 |x+3|^3 \ln |x+3|$$

4 (2+2)

Laplace transform to solve the initial value problem:

$$y''(t) + 4y(t) = f(t) + \delta(t - 1.5); \quad y(0) = 0, \quad y'(0) = 0;$$

where

$$f(t) = \begin{cases} 0 & 0 \leq t < 4 \\ (t-4)/6, & 4 \leq t < 10, \\ 1, & t \geq 10. \end{cases}$$

[20]

Let $Y = \mathcal{L}\{y\}$.

$$f(t) = ((t-4)/6) (u_4(t) - u_{10}(t)) + 1 \times u_{10}(t)$$

$$= (\frac{1}{6}(t-4)) u_4(t) + (-\frac{1}{6}(t-10)) u_{10}(t)$$

4'

$$s^2 Y - sy(0) - y'(0) + 4Y = (s^2 + 4) Y$$

$$= \mathcal{L}\{f(t)\} + \mathcal{L}\{\delta(t-1.5)\}$$

$$= e^{-4s} \cdot \frac{1}{6} \frac{1}{s^2} + e^{-10s} \cdot (-\frac{1}{6} \frac{1}{s^2}) + e^{-1.5s}$$

4'

$$\Rightarrow Y = \frac{e^{-4s}}{6s^2(s^2+4)} - \frac{1}{6s^2(s^2+4)} e^{-10s} + \frac{1}{s^2+4} e^{-1.5s}$$

4'

$$\frac{1}{s^2(s^2+4)} = \frac{1}{4} \left(\frac{1}{s^2} - \frac{1}{(s^2+4)} \right)$$

$$\Rightarrow \mathcal{L}^{-1} \left(\frac{1}{s^2(s^2+4)} \right) = \frac{1}{4} t - \frac{1}{8} \sin 2t$$

$$\mathcal{L}^{-1} \left(\frac{1}{s^2+4} \right) = \frac{1}{2} \sin 2t$$

$$\mathcal{L}^{-1} \left(\frac{1}{s^2(s^2+4)} e^{-4s} \right) = u_4(t) \left(\frac{1}{4} (t-4) - \frac{1}{8} \sin 2(t-4) \right)$$

$$\mathcal{L}^{-1} \left(\frac{1}{s^2(s^2+4)} e^{-10s} \right) = u_{10}(t) \left(\frac{1}{4} (t-10) - \frac{1}{8} \sin 2(t-10) \right)$$

6'

$$\mathcal{L}^{-1} \left(\frac{1}{s^2+4} e^{-1.5s} \right) = u_{1.5}(t) \frac{1}{2} \sin(2t-3)$$

Therefore

$$y = u_4(t) \left(\frac{1}{24} (t-4) - \frac{1}{48} \sin(2t-8) \right) - u_{10}(t) \left(\frac{1}{24} (t-10) - \frac{1}{48} \sin(2t-20) \right)$$

$$+ \frac{1}{2} u_{1.5}(t) \sin(2t-3)$$

2'

□

Apply the Laplace transform to solve the initial value problem:

$$2y'' + y' + 2y = e^{2t}, \quad y(0) = 0, \quad y'(0) = 1.$$

[15]

Solution. Let $Y = \mathcal{L}\{y\}$.

Apply Laplace transform to both hands sides of the equation, we have :

$$2\mathcal{L}\{y''\} + \mathcal{L}\{y'\} + 2Y = \frac{1}{s-2}$$

$$\Rightarrow 2(s^2 Y - s y(0) - y'(0)) + (sY - y(0)) + 2Y = \frac{1}{s-2}$$

$$\text{Since } y(0) = 0, \quad y'(0) = 1,$$

$$\text{we have } 2s^2 Y - 2 + sY + 2Y = \frac{1}{s-2}$$

$$(2s^2 + s + 2)Y = 2 + \frac{1}{s-2} = \frac{2s-3}{s-2}$$

$$Y = \frac{2s-3}{(s-2)(2s^2+s+2)}$$

$$= \frac{A}{s-2} + \frac{Bs+C}{2s^2+s+2}$$

$$2(s^2 + \frac{1}{2}s + 1)$$

$$2(s^2 + \frac{1}{2}s + \frac{1}{16} + \frac{15}{16})$$

$$2(s + \frac{1}{4})^2 + \frac{15}{8}$$

$$= \frac{2As^2 + As + 2A + Bs^2 + Cs - 2Bs - 2C}{(s-2)(2s^2+s+2)}$$

$$= \frac{(2A+B)s^2 + (A-2B+C)s + 2A-2C}{(s-2)(2s^2+s+2)}$$

$$\Rightarrow \begin{cases} 2A+B=0 \\ A-2B+C=2 \\ 2A-2C=-3 \end{cases}$$

$$\Rightarrow \begin{cases} A = \frac{1}{12} \\ B = -\frac{1}{6} \\ C = \frac{19}{12} \end{cases}$$

$$\Rightarrow Y = \frac{1}{12} \cdot \frac{1}{s-2} + \frac{-\frac{1}{6}(s + \frac{1}{4} - \frac{39}{4})}{2[(s + \frac{1}{4})^2 + \frac{15}{16}]} = \frac{1}{12} \cdot \frac{1}{s-2} - \frac{1}{12} \left[\frac{s + \frac{1}{4}}{(s + \frac{1}{4})^2 + \frac{15}{16}} - \frac{39}{4} \cdot \frac{1}{(s + \frac{1}{4})^2 + \frac{15}{16}} \right]$$

$$\Rightarrow y = \mathcal{L}^{-1}\{Y\} = \frac{1}{12}e^{2t} - \frac{1}{12}e^{-\frac{1}{2}t} \cos(\frac{\sqrt{15}}{4}t) + \frac{39}{48} \cdot \frac{4}{\sqrt{15}} e^{-\frac{1}{2}t} \sin(\frac{\sqrt{15}}{4}t)$$

5. Solve the initial value problem:

$$x' = \begin{pmatrix} -1/2 & 1 \\ -1 & -1/2 \end{pmatrix} x; \quad x(0) = \begin{pmatrix} 1 \\ -1 \end{pmatrix}.$$

[15]

Solution. Let $A = \begin{pmatrix} -\frac{1}{2} & 1 \\ -1 & -\frac{1}{2} \end{pmatrix}$.

$$\det(A - rI) = \det \begin{pmatrix} -\frac{1}{2} - r & 1 \\ -1 & -\frac{1}{2} - r \end{pmatrix} = \left(\frac{1}{2} - r\right)^2 + 1 = 0.$$

$$\Rightarrow r_1 = -\frac{1}{2} + i, \quad r_2 = -\frac{1}{2} - i$$

For $r_1 = -\frac{1}{2} + i$, let $\vec{\xi} = \begin{pmatrix} \xi_1 \\ \xi_2 \end{pmatrix}$,

$$\text{let } (A - r_1 I) \vec{\xi} = \begin{pmatrix} -i & 1 \\ -1 & -i \end{pmatrix} \begin{pmatrix} \xi_1 \\ \xi_2 \end{pmatrix} = \begin{pmatrix} 0 \\ 0 \end{pmatrix},$$

then $-i\xi_1 + \xi_2 = 0 \Rightarrow \xi_2 = i\xi_1 \Rightarrow \vec{\xi} = \begin{pmatrix} \xi_1 \\ i\xi_1 \end{pmatrix}$.

Choose $\vec{\xi} = \begin{pmatrix} 1 \\ i \end{pmatrix}$.

$$\begin{aligned} \text{The } \vec{\xi} \cdot e^{r_1 t} &= \begin{pmatrix} 1 \\ i \end{pmatrix} e^{(-\frac{1}{2} + i)t} = e^{-\frac{1}{2}t} \begin{pmatrix} 1 \\ i \end{pmatrix} (\cos t + i \sin t) \\ &= e^{-\frac{1}{2}t} \begin{pmatrix} \cos t + i \sin t \\ i \cos t - \sin t \end{pmatrix} \end{aligned}$$

$$\operatorname{Re}\{\vec{\xi} e^{r_1 t}\} = e^{-\frac{1}{2}t} \begin{pmatrix} \cos t \\ -\sin t \end{pmatrix}, \quad \operatorname{Im}\{\vec{\xi} e^{r_1 t}\} = e^{-\frac{1}{2}t} \begin{pmatrix} \sin t \\ \cos t \end{pmatrix}$$

So the general solution is

$$\vec{x} = e^{-\frac{1}{2}t} \left[c_1 \begin{pmatrix} \cos t \\ -\sin t \end{pmatrix} + c_2 \begin{pmatrix} \sin t \\ \cos t \end{pmatrix} \right]$$

Since $\vec{x}(0) = \begin{pmatrix} 1 \\ -1 \end{pmatrix} = c_1 \begin{pmatrix} 1 \\ 0 \end{pmatrix} + c_2 \begin{pmatrix} 0 \\ 1 \end{pmatrix}$,

we have $c_1 = 1, c_2 = -1$

$$\text{So } \vec{x} = e^{-\frac{1}{2}t} \left[\begin{pmatrix} \cos t \\ -\sin t \end{pmatrix} - \begin{pmatrix} \sin t \\ \cos t \end{pmatrix} \right] = e^{-\frac{1}{2}t} \begin{pmatrix} \cos t - \sin t \\ -\sin t - \cos t \end{pmatrix}$$

6. Consider the initial value problem:

$$y'' + y' - 6y = 0; \quad y(0) = 3, \quad y'(0) = 0.$$

- (a) Transform the problem into an initial value problem of first-order system of equations.
(b) Solve the initial value problem obtained in (a) using the method for systems of first-order equations.
(c) Find the solution y of the original initial value problem through the results obtained in (a) and (b).

[20]

(a) Let $y = x_1$; $y' = x_2$

Then $x_1' = y' = x_2$

$$x_2' + x_2 - 6x_1 = 0$$

Let $\vec{x} = (x_1, x_2)^T$

Therefore, $\vec{x}' = \begin{pmatrix} x_1' \\ x_2' \end{pmatrix} = \begin{pmatrix} x_2 \\ 6x_1 - x_2 \end{pmatrix} = A\vec{x}, \quad \vec{x}(0) = \begin{pmatrix} 3 \\ 0 \end{pmatrix}$

where $A = \begin{pmatrix} 0 & 1 \\ 6 & -1 \end{pmatrix}$

b) $\det(A - rI) = \begin{vmatrix} -r & 1 \\ 6 & -1-r \end{vmatrix} = r^2 + r - 6 = (r+3)(r-2)$

$$\Rightarrow r_1 = -3, \quad r_2 = 2$$

$$\Rightarrow (A + 3I) \vec{z}_1 = \begin{pmatrix} 3 & 1 \\ 6 & 2 \end{pmatrix} \begin{pmatrix} z_1 \\ z_2 \end{pmatrix} = \begin{pmatrix} 0 \\ 0 \end{pmatrix}$$

$$3z_1 + z_2 = 0 \quad \Rightarrow \quad \vec{z}_1 = (1, -3)^T$$

$$(A - 2I) \vec{z}_2 = \begin{pmatrix} -2 & 1 \\ 6 & -3 \end{pmatrix} \begin{pmatrix} z_1 \\ z_2 \end{pmatrix} = \begin{pmatrix} 0 \\ 0 \end{pmatrix}$$

$$-2z_1 + z_2 = 0 \quad \Rightarrow \quad \vec{z}_2 = (1, 2)^T$$

general solution: $\vec{x} = c_1 e^{-3t} \begin{pmatrix} 1 \\ -3 \end{pmatrix} + c_2 e^{2t} \begin{pmatrix} 1 \\ 2 \end{pmatrix}$

$$\vec{x}(0) = \begin{pmatrix} c_1 + c_2 \\ -3c_1 + 2c_2 \end{pmatrix} = \begin{pmatrix} 3 \\ 0 \end{pmatrix} \Rightarrow \begin{cases} c_1 = \frac{6}{5} \\ c_2 = \frac{9}{5} \end{cases}$$

$$\Rightarrow \vec{x} = \frac{6}{5} e^{-3t} \begin{pmatrix} 1 \\ -3 \end{pmatrix} + \frac{9}{5} e^{2t} \begin{pmatrix} 1 \\ 2 \end{pmatrix}$$

(c) $y = x_1 = \frac{6}{5} e^{-3t} + \frac{9}{5} e^{2t}$